pcuic/theories/PCUICClosed.v
@@ -392,9 +392,9 @@ Proof.
     + solve_all. unfold test_snd. simpl in *.
       toProp; eauto.
     + apply closedn_mkApps; auto.
-      rewrite forallb_app. simpl. rewrite H3.
+      rewrite forallb_app. simpl. rewrite H2.
       rewrite forallb_skipn; auto.
-      now apply closedn_mkApps_inv in H7.
+      now apply closedn_mkApps_inv in H6.
 
   - intuition auto.
     apply closedn_subst0.
